
$$\sum_{yjt} (C_{yjt}^{f} { ^.} S_{yjt} { ^.} A_{yjt}) + \sum_{yt} (C_{yt}^{s} { ^.} R_{yt}) + \sum_{yj} (C_{yj}^{u} { ^.} U_{yj})$$

$$ R_{yt} = R_{(y-1)t} + H_{yt} - L_{yt} $$

$$ R_{(y-1)t} - R_{yt} + H_{yt} - L_{yt} = 0 $$

$$ R_{t,1} = R_{t,0} + H_{t,1} - L_{t,1} $$

$$ R_{t,1} - H_{t,1} + L_{t,1} =  R_{t,0} $$

$$ L_{yt} = E_{yt} + \sum_{yif}^{f=t} (P_{yif} { ^.} H_{yi} ) $$

$$ L_{yt} - \sum_{yif}^{f=t} (P_{yif} { ^.} H_{yi}) = E_{yt} $$

$$ \sum_t (S_{yjt} { ^.} A_{yjt}) + U_{yj} \geq D_{yj} $$

$$ \sum_t (S_{yjt} { ^.} A_{yjt}) \geq D_{yj} $$

$$ \sum_{yjt=disallowed} A_{yjt} = 0 $$

$$ \sum_j A_{yjt} \leq R_{yt} $$

$$ \sum_j A_{yjt} - R_{yt} \leq 0 $$

$$ \sum_j (S_{yt} { ^.} A_{yjt}) \geq M_{yt} { ^.} R_{yt} $$

$$ \sum_j (S_{yt} { ^.} A_{yjt}) - M_{yt} { ^.} R_{yt} \geq 0 $$

$$ H_{yt} \leq C_{yt} $$

$$ S_{yjt} { ^.} A_{yjt} \geq P_{yjt} { ^.} D_{yj} $$

$$ S_{yjt} { ^.} A_{yjt} \leq {\breve{P}}_{yjt} { ^.} D_{yj} $$

\bye{document}
